BooleanAlgebraAxioms.v
@@ -1,28 +1,33 @@
 Set Implicit Arguments.
 
 Require Import Syntax.
-Require Import Sets.
 Require Import Semantics.
 Require Import Coq.Arith.EqNat.
 Require Import Coq.Classes.Equivalence.
 Require Import Coq.Classes.RelationClasses.
 Require Import Coq.Setoids.Setoid.
+Require Import Coq.Sets.Ensembles.
+Require Import Coq.Sets.Constructive_sets.
 Open Local Scope equiv_scope.
 Hint Resolve reflexivity.
 
-Existing Instances Set_equiv.
+Lemma union_set_subset_is_set :
+  forall (A : Type) (seta setb: Ensemble A), @Included _ seta setb -> @Union _  seta setb  = seta.
+Proof with auto. 
+  intros. unfold Included in *. 
+  Print Union.
+  apply Union_introl. 
 Lemma pred_null_or_single :
   forall (pred1 : exp) (h : history), (pred pred1) -> 
-         (eval pred1 h) === @empty history \/ (eval pred1 h) === (singleton h).
+         (eval pred1 h) = @Empty_set history \/ (eval pred1 h) = (Singleton _ h).
 Proof with auto. intros. 
   induction pred1; simpl; auto. 
-  left. reflexivity.
-  right. reflexivity.
-  destruct beq_nat. right. reflexivity. left. reflexivity.
-  inversion H. subst. apply IHpred1_1 in H2. apply IHpred1_2 in H3.
-  destruct H2; destruct H3. left. rewrite -> H0.
+  destruct beq_nat...
+  inversion H. subst. 
+  apply IHpred1_1 in H2. apply IHpred1_2 in H3.
+  destruct H2; destruct H3. rewrite H0. rewrite H1. auto. left. rewrite -> H0.
   rewrite -> H1. simpl.
-    
+  apply Union_inv.    
 left. simpl. reflexivity.
 
 Lemma ba_plus_one : 
