Sets.v
@@ -1,7 +1,94 @@
 Set Implicit Arguments.
+Require Import CpdtTactics.
 Require Import Coq.Classes.Equivalence.
 Require Import Coq.Classes.Morphisms.
 Require Import Coq.Setoids.Setoid.
+
+Module Type SETS.
+
+  Parameter t : Type. (* type of sets *)
+
+  Parameter elt : Type.
+
+  Parameter singleton : elt -> t.
+
+  Parameter empty : t.
+
+  Parameter union : t -> t -> t.
+
+  Parameter diff : t -> t -> t.
+
+  Parameter indexed_union : (nat -> t) -> t.
+
+  Parameter filter : (elt -> bool) -> t -> t.
+
+  Parameter map : (elt -> elt) -> t -> t
+
+  Parameter subset : t -> t -> Prop.
+
+  Parameter In : elt -> t -> Prop.
+
+  Axiom empty_spec : forall (x : elt), In x empty -> False.
+
+  Axiom singleton_spec : forall (x y : elt), In x (singleton y) <-> x = y.
+
+  Axiom union_intro_l : forall (x : elt) (s1 s2 : t), In x s1 -> In x (union s1 s2).
+  Axiom union_intro_r : forall (x : elt) (s1 s2 : t), In x s2 -> In x (union s1 s2).
+  Axiom union_extro : forall (x : elt) (s1 s2 : t), In x (union s1 s2) -> In x s1 \/ In x s2.
+
+  Axiom union_spec : forall (x : elt) (s1 s2 : t), In x (union s1 s2) <-> In x s1 \/ In x s2.
+
+  Axiom diff_spec : forall (x : elt) (s1 s2 : t), In x (diff s1 s2) <-> (In x s1 /\ ~(In x s2)).
+
+  Axiom subset_spec : forall (s1 s2 : t), subset s1 s2 <-> (forall (x : elt), In x s1 -> In x s2).
+
+  Axiom extensionality : forall (s1 s2 : t), (forall (x : elt), In x s1 <-> In x s2) -> s1 = s2.
+
+  Hint Resolve union_intro_l union_intro_r union_extro.
+  Hint Resolve empty_spec singleton_spec diff_spec subset_spec union_spec.
+
+  Hint Rewrite union_spec subset_spec singleton_spec.
+
+  Lemma union_comm : forall (s1 s2 : t), union s1 s2 = union s2 s1.
+  Proof with eauto.
+    intros.
+    apply extensionality.
+    intros.
+    autorewrite with core using simpl. intuition.
+  Qed.
+
+  Lemma union_assoc : forall (s1 s2 s3 : t), union s1 (union s2 s3) = union (union s1 s2) s3.
+  Proof with auto.
+    intros.
+    apply extensionality.
+    intros.
+    autorewrite with core using simpl. intuition.
+  Qed.
+
+  Lemma empty_is_subset : forall (s1 : t), subset empty s1. 
+  Proof with auto.
+   intros. 
+   apply subset_spec. intros.
+   apply empty_spec in H. contradiction.
+  Qed.
+
+  Lemma union_subset : forall (s1 s2 :t), subset s1 s2 -> (union s1 s2) = s2.
+  Proof with auto.
+   intros. 
+   apply extensionality.
+   intros.
+   rewrite subset_spec in H.
+   autorewrite with core using simpl.
+   intuition.
+  Qed. 
+
+  Lemma self_subset_self : forall (s1 : t), subset s1 s1.
+  Proof with auto.
+   intros. rewrite subset_spec. intros. intuition.
+  Qed. 
+
+ 
+
 
 Section Sets.
   
