tmp.v
@@ -1,0 +1,5 @@
+Set Implicit Arguments.
+
+Require Import Coq.Sets.Ensembles.
+
+Check In.
